Add weakened form of add step

src/Core.v
@@ -250,6 +250,31 @@ Record cfg_add_event_gen e r w W1 W2 :=
   wf_new_conf : wf X';
 }.
 
+Record cfg_add_event_struct e :=
+{ caes_e_new : E' ≡₁ E ∪₁ (eq e);
+  caes_e_notin : ~(E e);
+  caes_e_notinit : ~ is_init e;
+  caes_e_correct : new_event_correct e;
+  caes_wf_new_conf : wf X';
+  caes_cmt_graph_same : GC' = GC;
+}.
+
+Record cfg_add_event_props e r w W1 W2 :=
+{ caep_rf_new : rf G' ≡ rf G ∪ rf_delta_R GC e w ∪ rf_delta_W GC e (cmt ∩₁ E);
+  caep_co_new : co G' ≡ co G ∪ co_delta GC e W1 W2;
+  caep_rmw_new : rmw G' ≡ rmw G ∪ rmw_delta GC e r;
+}.
+
+Lemma cfg_add_event_iff_struct_and_props e r w W1 W2 :
+  cfg_add_event_gen e r w W1 W2 <->
+    << STRUCT : cfg_add_event_struct e >> /\
+    << PROPS : cfg_add_event_props e r w W1 W2 >>.
+Proof using.
+  split; [intros STEP | intros STRUPROPS].
+  { split; constructor; ins; apply STEP. }
+  constructor; ins; apply STRUPROPS.
+Qed.
+
 Definition cfg_add_event (e : actid) :=
   exists r w W1 W2, cfg_add_event_gen e r w W1 W2.
 
